FormaleSystemeInLean/LectureAndExercise/Fintype.lean
@@ -1,0 +1,35 @@
+-- inspired by mathlib
+class Fintype (α : Type u) where
+  elems : List α
+  complete : ∀ a : α, a ∈ elems
+
+def subtype_of_list (l : List α) := { x : α // x ∈ l }
+
+instance (l : List α) : Fintype (subtype_of_list l) where
+  elems := l.attach
+  complete := by
+    intro a
+    rcases a with ⟨p, v⟩
+    simp only [List.attach, subtype_of_list, List.attachWith]
+    grind
+
+instance (T : Fintype α) : Fintype (Option α) where
+  elems := T.elems.map (some · ) ++ [.none]
+  complete := by
+    intro a
+    simp only [List.mem_append, List.mem_map, List.mem_cons, List.not_mem_nil, or_false]
+    have some_mem (b : α) : some b ∈ T.elems.map (some · ) ++ [.none] := by
+      simp only [List.mem_append, List.mem_map, Option.some.injEq, exists_eq_right, List.mem_cons, reduceCtorEq, List.not_mem_nil, or_false]
+      exact T.complete b
+    by_cases hq : a = none
+    . apply Or.inr; exact hq
+    . rw [← Ne.eq_1, Option.ne_none_iff_exists] at hq
+      rcases hq with ⟨r, r_eq⟩
+      apply Or.inl
+      exists r
+      constructor
+      . exact T.complete r
+      . exact r_eq
+
+instance [Fintype α] [DecidableEq α] (l : List α) : BEq (subtype_of_list l) where
+  beq := fun q r => if q.val = r.val then true else false
